Metamath/VerifyDoneThms.lean
@@ -76,8 +76,8 @@ theorem done_parseErrorCode?_ws
           | .ax => some .unclosedAx
           | .thm => some .unclosedThm
       | .label _ _ => some .notACommand
-      | .includePath _ => some .notACommand
-      | .includeClose _ _ => some .notACommand
+      | .includePath _ _ => some .notACommand
+      | .includeClose _ _ _ => some .notACommand
       | .proof _ => some .unclosedProof := by
   unfold ParserState.done
   simp [h_charp, h_no_err, DB.error, DB.parseErrorCode?, DB.mkParseError, DB.mkErrorFromEvidence,
@@ -93,9 +93,9 @@ theorem done_parseErrorCode?_ws
       simp
   case label pos lab =>
     simp [ErrorEvidence.code, TokenFormError.code]
-  case includePath pos =>
+  case includePath resume pos =>
     simp [ErrorEvidence.code, TokenFormError.code]
-  case includeClose pos path =>
+  case includeClose resume pos path =>
     simp [ErrorEvidence.code, TokenFormError.code]
 
 /-- EOF inversion (token case): `done` returns the code dictated by the parser mode after
@@ -120,8 +120,8 @@ theorem done_parseErrorCode?_token
           | .ax => some .unclosedAx
           | .thm => some .unclosedThm
       | TokenParser.label _ _ => some .notACommand
-      | TokenParser.includePath _ => some .notACommand
-      | TokenParser.includeClose _ _ => some .notACommand
+      | TokenParser.includePath _ _ => some .notACommand
+      | TokenParser.includeClose _ _ _ => some .notACommand
       | TokenParser.proof _ => some .unclosedProof := by
   unfold ParserState.done
   simp [h_charp, h_no_err, h_feed_no_err, DB.error, DB.parseErrorCode?, DB.mkParseError,
@@ -137,9 +137,9 @@ theorem done_parseErrorCode?_token
       simp
   case label pos lab =>
     simp [ErrorEvidence.code, TokenFormError.code]
-  case includePath pos =>
+  case includePath resume pos =>
     simp [ErrorEvidence.code, TokenFormError.code]
-  case includeClose pos path =>
+  case includeClose resume pos path =>
     simp [ErrorEvidence.code, TokenFormError.code]
 
 end Verify
