test_databases/include_splicing/compressed_main.mm
@@ -1,0 +1,5 @@
+$c wff $.
+$v x $.
+vx $f wff x $.
+ax $a wff x $.
+th $p wff x $= ( ax ) A $[ compressed_child.mm $]
