test_databases/include_splicing/djvars_accept_main.mm
@@ -1,0 +1,3 @@
+$c wff $.
+$v x y $.
+$d x $[ djvars_accept_child.mm $]
