test_databases/include_splicing/djvars_empty_main.mm
@@ -1,0 +1,3 @@
+$c wff $.
+$v x $.
+$d x $[ djvars_empty_child.mm $]
